More

Cpc/Logos.lean
@@ -8380,9 +8380,9 @@ def __eo_is_closed_rec : Term -> Term -> Term
   | (Term.Apply (Term.Apply (Term.UOp UserOp.forall) vs) x), env => (__eo_is_closed_rec x (__eo_list_concat Term.__eo_List_cons vs env))
   | (Term.Apply (Term.Apply (Term.UOp UserOp.exists) vs) x), env => (__eo_is_closed_rec x (__eo_list_concat Term.__eo_List_cons vs env))
   | (Term.Apply f x), env => (__eo_and (__eo_is_closed_rec f env) (__eo_is_closed_rec x env))
-  | (Term.UOp1 u x), env => (__eo_is_closed_rec x env)
-  | (Term.UOp2 u x x2), env => (__eo_and (__eo_is_closed_rec x env) (__eo_is_closed_rec x2 env))
-  | (Term.UOp3 u x x2 x3), env => (__eo_and (__eo_and (__eo_is_closed_rec x env) (__eo_is_closed_rec x2 env)) (__eo_is_closed_rec x3 env))
+  | (Term.UOp1 u x), env => (__eo_is_closed_rec x Term.__eo_List_nil)
+  | (Term.UOp2 u x x2), env => (__eo_and (__eo_is_closed_rec x Term.__eo_List_nil) (__eo_is_closed_rec x2 Term.__eo_List_nil))
+  | (Term.UOp3 u x x2 x3), env => (__eo_and (__eo_and (__eo_is_closed_rec x Term.__eo_List_nil) (__eo_is_closed_rec x2 Term.__eo_List_nil)) (__eo_is_closed_rec x3 Term.__eo_List_nil))
   | x, env => (Term.Boolean true)
 
 
